\begin{enumerate}[label=\thesubsection.\arabic*,ref=\thesubsection.\theenumi]
    \item The sum of series $\frac{1}{2!}-\frac{1}{3!}+\frac{1}{4!}-\dots$ upto infinity is 
    \hfill(2007)
%
    \begin{enumerate}
    \item$e^{-\frac{1}{2}}$
    \item$e^{+\frac{1}{2}}$
    \item$e^{-2}$
    \item$e^{-1}$
    \end{enumerate}
\item For a positive integer $n$,  let
$a_n=1+\frac{1}{2}+\frac{1}{3}+\frac{1}{4}+\dots+\frac{1}{(2^n)-1}$. Then \hfill\brak{1999}
\begin{multicols}{4}
\begin{enumerate}    
\item $a100)\leq 100$
\item $a(100) > 100$
\item $a(200)\leq 100$
\item $a(200) > 100$
\end{enumerate}
\end{multicols}
%
%
\item Let 
\begin{align*}
S_n=\sum_{k=1}^{n}\frac{n}{n^2+kn+k^2} \text{ and }   T_n=\sum_{k=0}^{n-1}\frac{n}{n^2+kn+k^2}
\end{align*}
for $n=1, 2, 3, \dots$ Then, \hfill\brak{2008}
\begin{multicols}{4}
\begin{enumerate}    
\item $S_n<\frac{\pi}{3\sqrt{3}}$
\item $S_n>\frac{\pi}{3\sqrt{3}}$
\item $T_n<\frac{\pi}{3\sqrt{3}}$
\item $T_n>\frac{\pi}{3\sqrt{3}}$
\end{enumerate}
\end{multicols}
%
\end{enumerate}
