\begin{enumerate}[label=\thesubsection.\arabic*,ref=\thesubsection.\theenumi]
	\item The $n^{th}$ term of a GP is given by 
\begin{align}
	\label{eq:gp-nthterm}
	x(n)= x(0)r^n, n = 0,1,2, \dots 
\end{align}
where $r$
		is defined to be the {\em common ratio}.
\item Find the sum 
\begin{align}
	\label{eq:gp-sum10}
	S = 1 + 2 + 2^2 + 2^3 + 2^4
\end{align}
	\solution
Mulitpying the sum in
	\eqref{eq:gp-sum10}
	as
\begin{align}
	\label{eq:gp-sum10-rev}
	2S =  2 + 2^2 + 2^3 + 2^4+ 2^5
\end{align}
and  subtracting
	\eqref{eq:gp-sum10}
	from
	\eqref{eq:gp-sum10-rev},
\begin{align}
	\label{eq:gp-sum10-add}
	S = 2^5 - 1
\end{align}
\item The sum of a GP is 
\begin{align}
	 y(n)=\sum_{k=0}^{n-1}x(k)  
	= x(0)\brak{\frac{1-r^{n}}{1-r}}
	\label{eq:gp-sumn}
\end{align}
\item  For an infinite GP, 
\begin{align}
	\lim_{r\to\infty}	y(n) = 
	 \brak{\frac{x(0)}{1-r}},\quad \abs{r} < 1
	\label{eq:gp-sumn-infty}
\end{align}
\end{enumerate}
