\begin{enumerate}[label=\thesubsection.\arabic*,ref=\thesubsection.\theenumi]
%
\item Find the sum to $n$ terms of the series
$n^2 + 2^n$
	\item Find the sum to $n$ terms of the series: $5+11+19+29+41+\dots$
	\item Find the sum to $n$ terms of the series whos $n^{th}$ term is $n\brak{n+3}$.
\item Find the sum to $n$ terms of each of the series
	\begin{multicols}{2}
		\begin{enumerate}[itemsep=1ex]
			\item $n\brak{n+2}$
			\item $n\brak{\frac{n^2+5}{4}}$
\item $1 \times 2 + 2 \times 3 + 3 \times 4 + 4 \times 5 +\dots $
\item $1 \times 2 \times 3 + 2 \times 3 \times 4 + 3 \times 4 \times 5 + \dots $
\item $3 \times 1^2 + 5 \times 2^2 + 7 \times 3^2 + \dots $
\item $\frac{1}{1 \times 2}+\frac{1}{2\times3}+\frac{1}{3\times4}+\dots $
\item $5^2 + 6^2 + 7^2 + \dots  + 20^2$
\item $3 \times 8 + 6 \times 11 + 9 \times 14 + \dots $
\item $1^2 + (1^2 + 2^2 ) + (1^2 + 2^2 + 3^2 ) + \dots $
\item $n (n+1) (n+4)$.
\item $(2 n - 1)^2$
\item $\brak{n-1}\brak{2-n}\brak{3+n}$
\end{enumerate}
\end{multicols}
\item Find the sum to $n$ terms of the following series
\begin{enumerate}
\item $a_n = (-1)^{n-1}5^{n+1}$
\item $a_n = (-1)^{n-1}n^3$
\item $a_n = \frac{n^2}{2^n}$
\end{enumerate}
\item Obtain the closed form expression for the following
\begin{enumerate}
\item $a_1 = 1, a_n = a_{n-1}+2 \quad \forall n > 1$
\item $a_1 = 3, a_n = 3a_{n-1}+2 \quad \forall n > 1$
\item $a_1 = a_2 = 2, a_n = a_{n-1}-1, n > 2$ 
\item The Pingala sequence, defined by $$a_n = a_{n-1}+a_{n-2}, \quad n>2,  a_1 = a_2=1$$ 
\end{enumerate}
\item Find the sum of the following series up to $n$ terms
$$\frac{1^3}{1}+\frac{1^3+2^2}{1+3}+\frac{1^3+2^3+3^3}{1+3+5}+\dots$$
\item Show that $$\frac{1 \times 2^2+ 2 \times 3^2+\dots+n \times (n+1)^2}{1^2 \times 2 + 2^2 \times 3 +\dots+n^2 \times (n+1)} = \frac{3n+5}{3n+1}.$$
\item Find the $20^{th}$ term of the series: $2 \times 4 + 4 \times 6 + 6 \times 8 + \dots  $ 
\item Find the sum of the first $n$ terms of the series: 3 + 7 + 13 + 21 + 31 + \dots, 
\item If $S_1, S_2, S_3$ are the sum of first $n$ natural numbers, their squares and their cubes, respectively, show that $$9 S_2^2 = S_3 \brak{1 + 8S_1}.$$
\end{enumerate}
